Minor tweaks.

examples/machine-code/hoare-triple/prog_armLib.sig
@@ -12,9 +12,13 @@ sig
     val arm_spec_m1          : string -> (thm * int * int option) *
                                          (thm * int * int option) option
 
+    val arm_spec_m           : string -> (thm * int * int option) *
+                                         (thm * int * int option) option
+
     val arm_tools            : decompiler_tools
     val arm_tools_no_status  : decompiler_tools
     val arm_tools_byte       : decompiler_tools
+    val arm_tools_mem        : decompiler_tools
 
     val arm_enc              : string -> string
 
